finished proving fundamental theorem. Changed proof of normalisation slightly. Cleaned up fundamental theorem proof. Slight structual changes to types. fixed bug in fill function. proved transitivity of step relation. removed unused Maps file. updated Makefile.

SystemF.v
@@ -4,13 +4,10 @@
 
 Set Warnings "-notation-overridden,-parsing,-deprecated-hint-without-locality".
 From Coq Require Import Strings.String.
-From SFN Require Import Maps.
 Require Import List.
 Import ListNotations.
 From stdpp Require Import gmap.
 From Autosubst Require Export Autosubst.
-
-Hint Resolve update_eq : core.
 
 (* Relation *)
 Definition relation (X : Type) := X -> X -> Prop.
@@ -62,8 +59,6 @@ Global Instance Ids_expr : Ids tm. derive. Defined.
 Global Instance Rename_expr : Rename tm. derive. Defined.
 Global Instance Subst_expr : Subst tm. derive. Defined.
 Global Instance SubstLemmas_expr : SubstLemmas tm. derive. Qed.
-
-Print Subst_expr.
 
 Declare Custom Entry sysf.
 Notation "<{ e }>" := e (e custom sysf at level 99).
@@ -144,6 +139,8 @@ Inductive eval_ctxt :=
 | AppRCtxt (K : eval_ctxt) (v: tm) (Hv: value v) : eval_ctxt
 | TAppCtxt (K : eval_ctxt) : eval_ctxt.
 
+Hint Constructors eval_ctxt : core.
+
 Fixpoint fill (K : eval_ctxt) (e : tm) : tm :=
 	match K with
 	| HoleCtxt => e
@@ -153,7 +150,7 @@ Fixpoint fill (K : eval_ctxt) (e : tm) : tm :=
 	| PairRCtxt K' v Hv => tm_pair v (fill K' e)
 	| AppLCtxt K' e' => tm_app (fill K' e) e'
 	| AppRCtxt K' v Hv => tm_app v (fill K' e)
-	| TAppCtxt K' => tm_tyabs (fill K' e)
+	| TAppCtxt K' => tm_tyapp (fill K' e)
 	end.
 
 Fixpoint compose (K K' : eval_ctxt) : eval_ctxt :=
@@ -196,6 +193,18 @@ Hint Constructors step : core.
 Notation multistep := (multi step).
 Notation "e1 '-->*' e2" := (multistep e1 e2) (at level 40).
 
+Lemma step_trans : forall e1 e2 e3,
+	e1 -->* e2 ->
+	e2 -->* e3 ->
+	e1 -->* e3.
+Proof.
+	intros e1 e2 e3 He1e2. 
+	induction He1e2 as [e | e e' e'' Hee' He'e'' IH].
+	- trivial.
+	- intros He''e3. apply IH in He''e3 as He'e3. 
+		apply multi_step with e'; assumption.
+Qed.
+
 Lemma fill_compose: forall e K K',
 	fill K (fill K' e) = fill (compose K K') e.
 Proof.
@@ -222,13 +231,37 @@ Proof.
 		+ assumption.
 Qed.
 
+Lemma eval_ctxt_hole: forall e,
+	<{ e }> = fill HoleCtxt <{ e }>.
+Proof. auto. Qed.
 
-Lemma step_trans : forall e1 e2 e3,
-	e1 -->* e2 ->
-	e2 -->* e3 ->
-	e1 -->* e3.
-Proof.
-Admitted.
+Lemma eval_ctxt_fst: forall e,
+	<{ fst e }> = fill (FstCtxt HoleCtxt) e.
+Proof. auto. Qed.
+
+Lemma eval_ctxt_snd: forall e,
+	<{ snd e }> = fill (SndCtxt HoleCtxt) e.
+Proof. auto. Qed.
+
+Lemma eval_ctxt_pair_left: forall e1 e2, 
+	<{ (- e1, e2 -) }> = fill (PairLCtxt HoleCtxt e2) e1.
+Proof. auto. Qed.
+
+Lemma eval_ctxt_pair_right: forall v1 e2 H,
+	<{(- v1, e2 -)}> = fill (PairRCtxt HoleCtxt v1 H) e2.
+Proof. auto. Qed.
+
+Lemma eval_ctxt_app_left: forall e1 e2,
+	tm_app e1 e2 = fill (AppLCtxt HoleCtxt e2) e1.
+Proof. auto. Qed.
+	
+Lemma eval_ctxt_app_right: forall v1 e2 H,
+	tm_app v1 e2 = fill (AppRCtxt HoleCtxt v1 H) e2.
+Proof. auto. Qed.
+
+Lemma eval_ctxt_tapp: forall e,
+	tm_tyapp e = fill (TAppCtxt HoleCtxt) e.
+Proof. auto. Qed.
 
 Definition normalises (e : tm) := exists v, value v /\ e -->* v.
 
@@ -342,14 +375,14 @@ Inductive has_type : varContext -> tm -> ty -> Prop :=
 	| T_Abs : forall Gamma T1 T2 e,
 		(T1 :: Gamma) |- e : T2 ->
 		has_type Gamma (tm_abs e) (Ty_Arrow T1 T2)
-	| T_App : forall T1 T2 Gamma e1 e2,
-		Gamma |- e1 : (T2 -> T1) ->
-		Gamma |- e2 : T2 ->
-		Gamma |- e1 e2 : T1
+	| T_App : forall Gamma T1 T2 e1 e2,
+		Gamma |- e1 : (T1 -> T2) ->
+		Gamma |- e2 : T1 ->
+		Gamma |- e1 e2 : T2
 	| T_TLam : forall Gamma T e,
 		has_type (subst (ren (+1)) <$> Gamma) e T ->
 		has_type Gamma (tm_tyabs e) (Ty_Abs T)
-	| T_TApp : forall T T' Gamma e,
+	| T_TApp : forall Gamma T T' e,
 		has_type Gamma e (Ty_Abs T) ->
 		has_type Gamma (tm_tyapp e) T.[T'/]
 
@@ -376,7 +409,7 @@ Example typing_nonexample_3 :
 Proof.
 	intros [T H]. inversion H; subst. inversion H2; subst.
 	inversion H4; subst. inversion H3; subst.
-	inversion H6; subst. inversion H5. apply (ty_not_eq T2 T3). assumption.
+	inversion H6; subst. inversion H5. apply (ty_not_eq T2 T0). assumption.
 Qed.
 (** [] *)
 
@@ -675,76 +708,75 @@ Proof.
 	    simplify_eq. cbn. apply IHG; assumption.
 Qed.
 
-Lemma ofc: forall e1 e2, 
-	<{ (- e1, e2 -) }> = fill (PairLCtxt HoleCtxt e2) e1.
-Proof. reflexivity. Qed.
-
-Lemma ofc2: forall v1 e2 H,
-	value v1 ->
-	<{(- v1, e2 -)}> = fill (PairRCtxt HoleCtxt v1 H) e2.
-Proof. auto. Qed.
-
-Lemma ofc3: forall e,
-	<{ fst e }> = fill (FstCtxt HoleCtxt) e.
-Proof. auto. Qed.
-
-Lemma ofc4: forall v1 v2,
-	value v1 ->
-	value v2 ->
-	<{ fst (- v1, v2 -) }> = fill HoleCtxt <{fst (- v1, v2 -)}>.
-Proof. auto. Qed.
-
-Lemma ofc_v: forall v,
-	value v ->
-	<{ v }> = fill HoleCtxt <{ v }>.
-Proof. auto. Qed.
-
-Lemma ofc3_2: forall e,
-	<{ snd e }> = fill (SndCtxt HoleCtxt) e.
-Proof. auto. Qed.
-
-Lemma ofc4_2: forall v1 v2,
-	value v1 ->
-	value v2 ->
-	<{ snd (- v1, v2 -) }> = fill HoleCtxt <{ snd (- v1, v2 -)}>.
-Proof. auto. Qed.
-
 Theorem fundamental_theorem : forall Gamma e T,
 	Gamma |- e : T ->
 	log_rel Gamma e T.
 Proof with auto.
 	unfold log_rel.
 	intros Gamma e T HGeT xi vs Hxi_val. revert vs xi Hxi_val.
-	induction HGeT; intros vs xi Hxi_val Hlrs_xi_G_vs.
+	induction HGeT as [ Gamma x T HxGamma | Gamma 
+					  | Gamma T1 T2 e1 e2 HGe1T1 IH1 HGe2T2 IH2 
+					  | Gamma T1 T2 e HGeT1T2 IH 
+					  | Gamma T1 T2 e HGeT1T2 IH
+					  | Gamma T1 T2 e HGeT2 IH
+					  | Gamma T1 T2 e1 e2 HGe1T1T2 IH1 HGe2T2 IH2
+					  | Gamma T e HGeT IH
+					  | Gamma T T' e HGeAT IH].
+	all: intros vs xi Hxi_val Hlrs_xi_G_vs;
+	asimpl. (* The asimpl performs the substitution in the goals*)
 	- apply subst_step_var with Gamma; assumption.
-	- asimpl. exists tm_unit; done.
-	- asimpl. rewrite ofc. apply norm_bind with (lr_val xi T1).
-		split. apply IHHGeT1...
+	- exists tm_unit; done.
+	- rewrite eval_ctxt_pair_left. apply norm_bind with (lr_val xi T1).
+		split. apply IH1...
 		intros v1 (Hv1val & Hlrv_v1). cbn.
-		rewrite ofc2 with _ _ Hv1val...
+		rewrite eval_ctxt_pair_right with _ _ Hv1val...
 		apply norm_bind with (lr_val xi T2).
-		split. apply IHHGeT2...
+		split. apply IH2...
 		intros v2 (Hv2val & Hlrv_v2).
 		apply norm_val; cbn; auto.
 		exists v1, v2...
-	- asimpl. rewrite ofc3. apply norm_bind with (lr_val xi (Ty_Prod T1 T2)).
-		split. apply IHHGeT...
+	- rewrite eval_ctxt_fst. apply norm_bind with (lr_val xi (Ty_Prod T1 T2)).
+		split. apply IH...
 		intros v (Hvval & Hlrv_v).
 		destruct Hlrv_v as (v1 & v2 & Heq & Hlrv_v1 & Hlrv_v2).
 		subst. inversion Hvval; subst. apply norm_step with v1. split; cbn.
-		+ rewrite ofc4, ofc_v...
+		+ rewrite (eval_ctxt_hole <{fst (- v1, v2 -)}>). 
+			rewrite (eval_ctxt_hole v1). auto.
 		+ apply norm_val...
-	- asimpl. rewrite ofc3_2. apply norm_bind with (lr_val xi (Ty_Prod T1 T2)).
-		split. apply IHHGeT...
+	- rewrite eval_ctxt_snd. apply norm_bind with (lr_val xi (Ty_Prod T1 T2)).
+		split. apply IH...
 		intros v (Hvval & Hlrv_v).
 		destruct Hlrv_v as (v1 & v2 & Heq & Hlrv_v1 & Hlrv_v2).
 		subst. inversion Hvval; subst. apply norm_step with v2. split; cbn.
-		+ rewrite ofc4_2, ofc_v...
+		+ rewrite (eval_ctxt_hole <{snd (- v1, v2 -)}>). 
+			rewrite (eval_ctxt_hole v2). auto.
 		+ apply norm_val...
-	- 
-	-
-	-
-	-
+	- apply norm_val... exists (e.[up (env_subst vs)]); split...
+		intros v' Hlrv_v'. asimpl. 
+		assert (Hes: v' .: env_subst vs = env_subst (v' :: vs))... 
+		rewrite Hes. apply IH... cbn. exists v', vs...
+	- rewrite eval_ctxt_app_left. 
+		apply norm_bind with (lr_val xi (Ty_Arrow T1 T2)).
+		split. apply IH1...
+		intros v1 (Hv1val & Hlrv_v1). destruct Hlrv_v1 as (e & Heq & H); subst.
+		cbn. rewrite eval_ctxt_app_right with _ _ Hv1val...
+		apply norm_bind with (lr_val xi T1). split. apply IH2...
+		intros v2 (Hv2val & Hlrv_v2). apply norm_step with e.[v2/]. split.
+		+ cbn. rewrite (eval_ctxt_hole (tm_app (tm_abs e) v2)). 
+			rewrite eval_ctxt_hole. auto.
+		+ apply (H v2 Hlrv_v2).
+	- apply norm_val... exists (e.[env_subst vs]). split...
+		intros P HovP. apply IH... apply log_rel_seq_weaken...
+	- rewrite eval_ctxt_tapp. apply norm_bind with (lr_val xi (Ty_Abs T)).
+		split. apply IH...
+		intros v (Hvval & Hlrv_v). destruct Hlrv_v as (e' & Heq & H); subst.
+		apply norm_step with e'. split.
+		+ cbn. rewrite (eval_ctxt_hole <{(/\ e') _}>). 
+			rewrite (eval_ctxt_hole e'). auto.
+		+ apply norm_mono with (lr_val ( (lr_val xi T' ) :: xi) T).
+			* intros v. apply log_rel_subst...
+			* apply (H (lr_val xi T')). intros v Hlrv_v. 
+				apply (lr_val_val xi T')...
 Qed.
 
 Theorem normalisation: forall e T,
@@ -752,10 +784,9 @@ Theorem normalisation: forall e T,
 	normalises e.
 Proof.
 	intros e T HT.
-	apply fundamental_theorem with (vs := []) (xi := []) in HT; cbn; auto.
-	unfold normalises_pred in HT.
-	asimpl in HT. destruct HT as [v [Hv [Hv' Hv'']]].
-	unfold normalises. eauto.
+	apply fundamental_theorem in HT. unfold log_rel in HT.
+	specialize HT with [] []. asimpl in HT. destruct HT as (v & Hvval & Hev & Hlrv_v).
+	1,2: done. exists v. split; done.
 Qed.
 
 End SystemF.
